Add oHD and oEL (option-valued) functions from CakeML
oEL was called LLOOKUP in CakeML but I don't much like that name.

src/list/src/listScript.sml
@@ -3751,6 +3751,65 @@ val TAKE_compute =
 val DROP_compute =
    Theory.save_thm("DROP_compute", numLib.SUC_RULE DROP_compute);
 
+(* ----------------------------------------------------------------------
+    versions of constants with option outputs rather than unspecified
+
+      oHD : 'a list -> 'a option
+      oEL : num -> 'a list -> 'a option
+
+   ---------------------------------------------------------------------- *)
+
+val oHD_def = Define`oHD l = case l of [] => NONE | h::_ => SOME h`
+val oHD_thm = Q.store_thm("oHD_thm[simp]",
+  `(oHD [] = NONE) /\ (oHD (h::t) = SOME h)`,
+  rw[oHD_def]);
+
+val oEL_def = Define`
+  (oEL n [] = NONE) /\
+  (oEL n (x::xs) = if n = 0 then SOME x else oEL (n - 1) xs)
+`;
+
+val oEL_THM = Q.store_thm(
+  "oEL_THM",
+  `!xs n. oEL n xs = if n < LENGTH xs then SOME (EL n xs) else NONE`,
+  Induct >> fs[oEL_def] >> rw[] >> fs[]
+  >- (Q.RENAME_TAC [‘n < SUC (LENGTH xs)’] >> Cases_on ‘n’ >> fs[]) >>
+  rw[] >> ASSUME_TAC (numLib.DECIDE “!x. 1 + x = SUC x”) >>
+  fs[arithmeticTheory.NOT_ZERO_LT_ZERO] >>
+  METIS_TAC[ONE, arithmeticTheory.LESS_LESS_SUC]);
+
+val oEL_EQ_EL = Q.store_thm(
+  "oEL_EQ_EL",
+  ‘!xs n y. (oEL n xs = SOME y) <=> n < LENGTH xs /\ (y = EL n xs)’,
+  simp[oEL_THM] >> METIS_TAC[]);
+
+val oEL_DROP = Q.store_thm(
+  "oEL_DROP",
+  ‘oEL n (DROP m xs) = oEL (m + n) xs’,
+  MAP_EVERY Q.ID_SPEC_TAC [‘n’, ‘m’, ‘xs’] >> Induct_on ‘xs’ >>
+  simp[DROP_def, oEL_def] >> rw[oEL_def] >> fs[] >>
+  Q.RENAME_TAC [‘m - 1 + n’] >>
+  ‘m - 1 + n = m + n - 1’ suffices_by simp[] >>
+  Q.UNDISCH_THEN ‘m <> 0’ MP_TAC >> numLib.ARITH_TAC);
+
+val oEL_TAKE_E = Q.store_thm(
+  "oEL_TAKE_E",
+  ‘(oEL n (TAKE m xs) = SOME x) ==> (oEL n xs = SOME x)’,
+  MAP_EVERY Q.ID_SPEC_TAC [‘n’, ‘m’, ‘xs’] >> Induct_on ‘xs’ >>
+  simp[TAKE_def, oEL_def] >> rw[oEL_def] >> RES_TAC);
+
+val oEL_LUPDATE = Q.store_thm(
+  "oEL_LUPDATE",
+  ‘!xs i n x. oEL n (LUPDATE x i xs) =
+               if i <> n then oEL n xs else
+               if i < LENGTH xs then SOME x else NONE’,
+  Induct >> fs[oEL_def,LUPDATE_def] >>
+  Cases_on ‘i’ >> rw[oEL_def,LUPDATE_def] >> fs[] >> rw[] >>
+  fs[numLib.DECIDE “!x. SUC (x - 1) <> x <=> (x = 0)”,
+     numLib.DECIDE “!x. 1 + x = SUC x”]);
+
+(* ---------------------------------------------------------------------- *)
+
 val _ = app DefnBase.export_cong ["EXISTS_CONG", "EVERY_CONG", "MAP_CONG",
                                   "MAP2_CONG", "EVERY2_cong", "FOLDL2_cong",
                                   "FOLDL_CONG", "FOLDR_CONG", "list_size_cong"]
